cedar-lean/Cedar/Thm.lean
@@ -14,6 +14,6 @@
  limitations under the License.
 -/
 
-import Cedar.Thm.Basic
+import Cedar.Thm.Authorization
 import Cedar.Thm.Slicing
-import Cedar.Thm.Soundness
+import Cedar.Thm.Typechecking
