cedar-lean/Cedar/Thm/Validation/Typechecker.lean
@@ -1,0 +1,101 @@
+/-
+ Copyright 2022-2023 Amazon.com, Inc. or its affiliates. All Rights Reserved.
+
+ Licensed under the Apache License, Version 2.0 (the "License");
+ you may not use this file except in compliance with the License.
+ You may obtain a copy of the License at
+
+      https://www.apache.org/licenses/LICENSE-2.0
+
+ Unless required by applicable law or agreed to in writing, software
+ distributed under the License is distributed on an "AS IS" BASIS,
+ WITHOUT WARRANTIES OR CONDITIONS OF ANY KIND, either express or implied.
+ See the License for the specific language governing permissions and
+ limitations under the License.
+-/
+
+import Cedar.Thm.Validation.Typechecker.And
+import Cedar.Thm.Validation.Typechecker.BinaryApp
+import Cedar.Thm.Validation.Typechecker.Call
+import Cedar.Thm.Validation.Typechecker.GetAttr
+import Cedar.Thm.Validation.Typechecker.HasAttr
+import Cedar.Thm.Validation.Typechecker.IfThenElse
+import Cedar.Thm.Validation.Typechecker.LitVar
+import Cedar.Thm.Validation.Typechecker.Record
+import Cedar.Thm.Validation.Typechecker.Set
+import Cedar.Thm.Validation.Typechecker.Or
+import Cedar.Thm.Validation.Typechecker.UnaryApp
+
+/-!
+This file contains useful definitions and lemmas about the `Typechecker` functions.
+-/
+
+namespace Cedar.Thm
+
+open Cedar.Data
+open Cedar.Spec
+open Cedar.Validation
+
+/--
+If an expression is well-typed according to the typechecker, and the input
+environment and capabilities satisfy some invariants, then either (1) evaluation
+produces a value of the returned type or (2) it returns an error of type
+`entityDoesNotExist`, `extensionError`, or `arithBoundsError`. Both options are
+encoded in the `EvaluatesTo` predicate.
+-/
+theorem type_of_is_sound {e : Expr} {c₁ c₂ : Capabilities} {env : Environment} {ty : CedarType} {request : Request} {entities : Entities} :
+  CapabilitiesInvariant c₁ request entities →
+  RequestAndEntitiesMatchEnvironment env request entities →
+  typeOf e c₁ env = .ok (ty, c₂) →
+  GuardedCapabilitiesInvariant e c₂ request entities ∧
+  ∃ (v : Value), EvaluatesTo e request entities v ∧ InstanceOfType v ty
+:= by
+  intro h₁ h₂ h₃
+  match e with
+  | .lit l => exact type_of_lit_is_sound h₃
+  | .var var => exact type_of_var_is_sound h₂ h₃
+  | .ite x₁ x₂ x₃ =>
+    rcases (@type_of_is_sound x₁) with ih₁
+    rcases (@type_of_is_sound x₂) with ih₂
+    rcases (@type_of_is_sound x₃) with ih₃
+    exact type_of_ite_is_sound h₁ h₂ h₃ ih₁ ih₂ ih₃
+  | .and x₁ x₂ =>
+    rcases (@type_of_is_sound x₁) with ih₁
+    rcases (@type_of_is_sound x₂) with ih₂
+    exact type_of_and_is_sound h₁ h₂ h₃ ih₁ ih₂
+  | .or x₁ x₂ =>
+    rcases (@type_of_is_sound x₁) with ih₁
+    rcases (@type_of_is_sound x₂) with ih₂
+    exact type_of_or_is_sound h₁ h₂ h₃ ih₁ ih₂
+  | .unaryApp op₁ x₁ =>
+    rcases (@type_of_is_sound x₁) with ih
+    exact type_of_unaryApp_is_sound h₁ h₂ h₃ ih
+  | .binaryApp op₂ x₁ x₂ =>
+    rcases (@type_of_is_sound x₁) with ih₁
+    rcases (@type_of_is_sound x₂) with ih₂
+    exact type_of_binaryApp_is_sound h₁ h₂ h₃ ih₁ ih₂
+  | .hasAttr x₁ a =>
+    rcases (@type_of_is_sound x₁) with ih
+    exact type_of_hasAttr_is_sound h₁ h₂ h₃ ih
+  | .getAttr x₁ a =>
+    rcases (@type_of_is_sound x₁) with ih
+    exact type_of_getAttr_is_sound h₁ h₂ h₃ ih
+  | .set xs =>
+    have ih : ∀ xᵢ, xᵢ ∈ xs → TypeOfIsSound xᵢ := by
+      intro xᵢ _
+      exact @type_of_is_sound xᵢ
+    exact type_of_set_is_sound h₁ h₂ h₃ ih
+  | .record axs =>
+    have ih : ∀ axᵢ, axᵢ ∈ axs → TypeOfIsSound axᵢ.snd := by
+      intro axᵢ hᵢ
+      have _ : sizeOf axᵢ.snd < 1 + sizeOf axs := by
+        apply List.sizeOf_snd_lt_sizeOf_list hᵢ
+      exact @type_of_is_sound axᵢ.snd
+    exact type_of_record_is_sound h₁ h₂ h₃ ih
+  | .call xfn xs =>
+    have ih : ∀ xᵢ, xᵢ ∈ xs → TypeOfIsSound xᵢ := by
+      intro xᵢ _
+      exact @type_of_is_sound xᵢ
+    exact type_of_call_is_sound h₁ h₂ h₃ ih
+termination_by
+  type_of_is_sound e c₁ c₂ env ty request entities _ _ _ => sizeOf e
