cedar-lean/Cedar/Thm/Validation/Typechecker/And.lean
@@ -1,0 +1,161 @@
+/-
+ Copyright 2022-2023 Amazon.com, Inc. or its affiliates. All Rights Reserved.
+
+ Licensed under the Apache License, Version 2.0 (the "License");
+ you may not use this file except in compliance with the License.
+ You may obtain a copy of the License at
+
+      https://www.apache.org/licenses/LICENSE-2.0
+
+ Unless required by applicable law or agreed to in writing, software
+ distributed under the License is distributed on an "AS IS" BASIS,
+ WITHOUT WARRANTIES OR CONDITIONS OF ANY KIND, either express or implied.
+ See the License for the specific language governing permissions and
+ limitations under the License.
+-/
+
+import Cedar.Thm.Validation.Typechecker.Basic
+
+/-!
+This file proves that typechecking of `.and` expressions is sound.
+-/
+
+namespace Cedar.Thm
+
+open Cedar.Data
+open Cedar.Spec
+open Cedar.Validation
+
+theorem type_of_and_inversion {x₁ x₂ : Expr} {c c' : Capabilities} {env : Environment} {ty : CedarType}
+  (h₁ : typeOf (Expr.and x₁ x₂) c env = Except.ok (ty, c')) :
+  ∃ bty₁ c₁,
+    typeOf x₁ c env = .ok (.bool bty₁, c₁) ∧
+    if bty₁ = BoolType.ff
+    then ty = .bool BoolType.ff ∧ c' = ∅
+    else ∃ bty₂ c₂,
+      typeOf x₂ (c ∪ c₁) env = .ok (.bool bty₂, c₂) ∧
+      if bty₂ = BoolType.ff
+      then ty = .bool BoolType.ff ∧ c' = ∅
+      else ty = .bool (lubBool bty₁ bty₂) ∧ c' = c₁ ∪ c₂
+:= by
+  simp [typeOf] at h₁
+  cases h₂ : typeOf x₁ c env <;> simp [h₂] at *
+  rename_i res₁
+  simp [typeOfAnd] at h₁
+  split at h₁ <;> simp [ok, err] at h₁
+  case ok.h_1 h₃ =>
+    exists BoolType.ff, res₁.snd ; simp [h₁]
+    simp at h₃
+    rcases h₁ with ⟨h₁, _⟩ ; subst h₁
+    rcases h₃ with ⟨h₃, _⟩
+    simp [←h₃]
+  case ok.h_2 bty₁ c₁ h₃ h₄ =>
+    exists bty₁, c₁
+    simp at h₄ ; rcases h₄ with ⟨hty₁, hc₁⟩ ; simp [←hty₁, ←hc₁]
+    split ; contradiction
+    cases h₄ : typeOf x₂ (c ∪ res₁.snd) env <;> simp [h₄] at *
+    rename_i res₂
+    split at h₁ <;> simp at h₁ <;>
+    rcases h₁ with ⟨hty, hc⟩ <;> subst hty hc
+    case h_1.intro hty₂ =>
+      exists BoolType.ff, res₂.snd ; simp [←hty₂]
+    case h_2.intro hty₂ =>
+      exists BoolType.tt, res₂.snd ; simp [←hty₂, hc₁]
+      cases bty₁ <;> simp at h₃ <;> simp [lubBool]
+    case h_3.intro bty₂ h₄ h₅ hty₂ =>
+      exists BoolType.anyBool, res₂.snd
+      cases bty₂ <;> simp at *
+      simp [←hty₂, hc₁, lubBool]
+      split
+      case inl h₆ => simp [h₆]
+      case inr => rfl
+
+theorem type_of_and_is_sound {x₁ x₂ : Expr} {c₁ c₂ : Capabilities} {env : Environment} {ty : CedarType} {request : Request} {entities : Entities}
+  (h₁ : CapabilitiesInvariant c₁ request entities)
+  (h₂ : RequestAndEntitiesMatchEnvironment env request entities)
+  (h₃ : typeOf (Expr.and x₁ x₂) c₁ env = Except.ok (ty, c₂))
+  (ih₁ : TypeOfIsSound x₁)
+  (ih₂ : TypeOfIsSound x₂) :
+  GuardedCapabilitiesInvariant (Expr.and x₁ x₂) c₂ request entities ∧
+  ∃ v, EvaluatesTo (Expr.and x₁ x₂) request entities v ∧ InstanceOfType v ty
+:= by
+  rcases (type_of_and_inversion h₃) with ⟨bty₁, rc₁, h₄, h₅⟩
+  specialize ih₁ h₁ h₂ h₄
+  rcases ih₁ with ⟨ih₁₁, v₁, ih₁₂, ih₁₃⟩
+  rcases (instance_of_bool_is_bool ih₁₃) with ⟨b₁, hb₁⟩ ; subst hb₁
+  split at h₅
+  case inl h₆ =>
+    subst h₆
+    rcases h₅ with ⟨hty, hc⟩ ; subst hty hc
+    apply And.intro
+    case left => exact empty_guarded_capabilities_invariant
+    case right =>
+      rcases (instance_of_ff_is_false ih₁₃) with h₇
+      simp at h₇ ; subst h₇
+      simp [EvaluatesTo] at ih₁₂
+      rcases ih₁₂ with ih₁₂ | ih₁₂ | ih₁₂ | ih₁₂ <;>
+      simp [EvaluatesTo, evaluate, Result.as, ih₁₂, Coe.coe, Value.asBool] <;>
+      try exact type_is_inhabited (CedarType.bool BoolType.ff)
+      exact false_is_instance_of_ff
+  case inr h₆ =>
+    rcases h₅ with ⟨bty₂, rc₂, h₅, h₇⟩
+    split at h₇ <;> rcases h₇ with ⟨hty, hc⟩ <;> subst hty hc
+    case inl.intro h₈ =>
+      subst h₈
+      apply And.intro
+      case left => exact empty_guarded_capabilities_invariant
+      case right =>
+        exists false ; simp [false_is_instance_of_ff]
+        cases b₁
+        case false =>
+          rcases ih₁₂ with ih₁₂ | ih₁₂ | ih₁₂ | ih₁₂ <;>
+          simp [EvaluatesTo, evaluate, Result.as, ih₁₂, Coe.coe, Value.asBool]
+        case true =>
+          rcases ih₁₂ with ih₁₂ | ih₁₂ | ih₁₂ | ih₁₂ <;>
+          simp [EvaluatesTo, evaluate, Result.as, ih₁₂, Coe.coe, Value.asBool]
+          simp [GuardedCapabilitiesInvariant] at ih₁₁
+          specialize ih₁₁ ih₁₂
+          rcases (capability_union_invariant h₁ ih₁₁) with h₇
+          specialize ih₂ h₇ h₂ h₅
+          rcases ih₂ with ⟨_, v₂, ih₂₂, ih₂₃⟩
+          simp [EvaluatesTo] at ih₂₂
+          rcases ih₂₂ with ih₂₂ | ih₂₂ | ih₂₂ | ih₂₂ <;>
+          simp [EvaluatesTo, evaluate, Result.as, ih₂₂, Coe.coe, Value.asBool]
+          rcases (instance_of_ff_is_false ih₂₃) with h₈
+          subst h₈ ; simp only
+    case inr.intro h₈ =>
+      cases b₁
+      case false =>
+        rcases ih₁₂ with ih₁₂ | ih₁₂ | ih₁₂ | ih₁₂ <;>
+        simp [EvaluatesTo, evaluate, Result.as, ih₁₂, Coe.coe, Value.asBool, GuardedCapabilitiesInvariant] <;>
+        try exact type_is_inhabited (CedarType.bool (lubBool bty₁ bty₂))
+        apply instance_of_lubBool ; simp [ih₁₃]
+      case true =>
+        rcases ih₁₂ with ih₁₂ | ih₁₂ | ih₁₂ | ih₁₂ <;>
+        simp [EvaluatesTo, evaluate, Result.as, ih₁₂, Coe.coe, Value.asBool, GuardedCapabilitiesInvariant] <;>
+        try exact type_is_inhabited (CedarType.bool (lubBool bty₁ bty₂))
+        simp [GuardedCapabilitiesInvariant] at ih₁₁
+        specialize ih₁₁ ih₁₂
+        rcases (capability_union_invariant h₁ ih₁₁) with h₇
+        specialize ih₂ h₇ h₂ h₅
+        rcases ih₂ with ⟨ih₂₁, v₂, ih₂₂, ih₂₃⟩
+        simp [EvaluatesTo] at ih₂₂
+        rcases ih₂₂ with ih₂₂ | ih₂₂ | ih₂₂ | ih₂₂ <;>
+        simp [EvaluatesTo, evaluate, Result.as, ih₂₂, Coe.coe, Value.asBool] <;>
+        try exact type_is_inhabited (CedarType.bool (lubBool bty₁ bty₂))
+        rcases (instance_of_bool_is_bool ih₂₃) with ⟨b₂, hb₂⟩ ; subst hb₂
+        cases b₂ <;> simp
+        case false =>
+          exists false ; simp only [true_and]
+          apply instance_of_lubBool ; simp [ih₂₃]
+        case true =>
+          apply And.intro
+          case left =>
+            simp [GuardedCapabilitiesInvariant] at ih₂₁
+            specialize ih₂₁ ih₂₂
+            exact capability_union_invariant ih₁₁ ih₂₁
+          case right =>
+            exists true ; simp only [true_and]
+            apply instance_of_lubBool ; simp [ih₁₃]
+
+end Cedar.Thm
