cedar-lean/Cedar/Thm/Validation/Typechecker/Basic.lean
@@ -1,0 +1,138 @@
+/-
+ Copyright 2022-2023 Amazon.com, Inc. or its affiliates. All Rights Reserved.
+
+ Licensed under the Apache License, Version 2.0 (the "License");
+ you may not use this file except in compliance with the License.
+ You may obtain a copy of the License at
+
+      https://www.apache.org/licenses/LICENSE-2.0
+
+ Unless required by applicable law or agreed to in writing, software
+ distributed under the License is distributed on an "AS IS" BASIS,
+ WITHOUT WARRANTIES OR CONDITIONS OF ANY KIND, either express or implied.
+ See the License for the specific language governing permissions and
+ limitations under the License.
+-/
+
+import Cedar.Spec
+import Cedar.Validation
+import Cedar.Thm.Core.Std
+import Cedar.Thm.Validation.Typechecker.Types
+
+/-!
+This file contains useful definitions and lemmas about the `Typechecker` functions.
+-/
+
+namespace Cedar.Thm
+
+open Cedar.Data
+open Cedar.Spec
+open Cedar.Validation
+
+/--
+The type soundness property says that if the typechecker assigns a type to an
+expression, then it must be the case that the expression `EvaluatesTo` a value
+of that type. The `EvaluatesTo` predicate covers the (obvious) case where
+evaluation has no errors, but it also allows for errors of type
+`entityDoesNotExist`, `extensionError`, and `arithBoundsError`.
+
+The typechecker cannot protect against these errors because they depend on
+runtime information (i.e., the entities passed into the authorization request,
+extension function applications on authorization-time data, and arithmetic
+overflow errors). All other errors (`attrDoesNotExist` and `typeError`) can be
+prevented statically.
+
+_Note_: Currently, `extensionError`s can also be ruled out at validation time
+because the only extension functions that can error are constructors, and all
+constructors are required to be applied to string literals, meaning that they
+can be fully evaluated during validation. This is not guaranteed to be the case
+in the future.
+
+_Note_: We plan to implement a range analysis that will be able to rule out
+`arithBoundsError`s.
+-/
+def EvaluatesTo (e: Expr) (request : Request) (entities : Entities) (v : Value) : Prop :=
+  evaluate e request entities = .error .entityDoesNotExist ∨
+  evaluate e request entities = .error .extensionError ∨
+  evaluate e request entities = .error .arithBoundsError ∨
+  evaluate e request entities = .ok v
+
+/--
+On input to the typechecking function, for any (e,k) in the Capabilities,
+e is a record- or entity-typed expression that has key k.
+-/
+def CapabilitiesInvariant (c : Capabilities) (request : Request) (entities : Entities) : Prop :=
+  ∀ (e : Expr) (k : Attr), (e, k) ∈ c → EvaluatesTo (.hasAttr e k) request entities true
+
+/--
+The Capabilities output by the typechecking function will satisfy
+`CapabilitiesInvariant` provided that the input expression evaluates to true.
+-/
+def GuardedCapabilitiesInvariant (e: Expr) (c: Capabilities) (request : Request) (entities : Entities) : Prop :=
+  evaluate e request entities = .ok true →
+  CapabilitiesInvariant c request entities
+
+def TypeOfIsSound (x₁ : Expr) : Prop :=
+  ∀ {c₁ c₂ : Capabilities} {env : Environment} {ty : CedarType} {request : Request} {entities : Entities},
+    CapabilitiesInvariant c₁ request entities →
+    RequestAndEntitiesMatchEnvironment env request entities →
+    typeOf x₁ c₁ env = Except.ok (ty, c₂) →
+    GuardedCapabilitiesInvariant x₁ c₂ request entities ∧
+    ∃ v, EvaluatesTo x₁ request entities v ∧ InstanceOfType v ty
+
+----- Capability lemmas -----
+
+theorem empty_capabilities_invariant (request : Request) (entities : Entities) :
+  CapabilitiesInvariant ∅ request entities
+:= by
+  intro e k h
+  contradiction
+
+theorem empty_guarded_capabilities_invariant {e: Expr} {request : Request} {entities : Entities} :
+  GuardedCapabilitiesInvariant e ∅ request entities
+:= by
+  intro _
+  exact empty_capabilities_invariant request entities
+
+theorem capability_implies_record_attribute {x₁ : Expr} {a : Attr} {c₁ : Capabilities} {request : Request} {entities : Entities} {r : Map Attr Value}
+  (h₁ : CapabilitiesInvariant c₁ request entities)
+  (h₂ : evaluate x₁ request entities = Except.ok (Value.record r))
+  (h₃ : (x₁, a) ∈ c₁) :
+  ∃ vₐ, r.find? a = some vₐ
+:= by
+  simp [CapabilitiesInvariant] at h₁
+  specialize h₁ x₁ a h₃
+  simp [EvaluatesTo, evaluate, h₂, hasAttr, attrsOf, Map.contains_iff_some_find?] at h₁
+  exact h₁
+
+theorem capability_implies_entity_attribute {x₁ : Expr} {a : Attr} {c₁ : Capabilities} {request : Request} {entities : Entities} {uid: EntityUID} {d: EntityData}
+  (h₁ : CapabilitiesInvariant c₁ request entities)
+  (h₂ : evaluate x₁ request entities = Except.ok (Value.prim (Prim.entityUID uid)))
+  (h₃ : Map.find? entities uid = some d)
+  (h₄ : (x₁, a) ∈ c₁) :
+  ∃ vₐ, d.attrs.find? a = some vₐ
+:= by
+  simp [CapabilitiesInvariant] at h₁
+  specialize h₁ x₁ a h₄
+  simp [EvaluatesTo, evaluate, h₂, hasAttr, attrsOf, Entities.attrsOrEmpty, h₃, Map.contains_iff_some_find?] at h₁
+  exact h₁
+
+theorem capability_union_invariant {c₁ c₂ : Capabilities} {request : Request} {entities : Entities}
+  (h₁ : CapabilitiesInvariant c₁ request entities)
+  (h₂ : CapabilitiesInvariant c₂ request entities) :
+  CapabilitiesInvariant (c₁ ∪ c₂) request entities
+:= by
+  simp [CapabilitiesInvariant] at *
+  intro x a h₃
+  specialize h₁ x a ; specialize h₂ x a
+  cases h₃ <;> rename_i h₃ <;> simp [h₃] at * <;> assumption
+
+theorem capability_intersection_invariant {c₁ c₂ : Capabilities} {request : Request} {entities : Entities}
+  (h₁ : CapabilitiesInvariant c₁ request entities ∨ CapabilitiesInvariant c₂ request entities) :
+  CapabilitiesInvariant (c₁ ∩ c₂) request entities
+:= by
+  simp [CapabilitiesInvariant] at *
+  intro x a h₃ h₄
+  cases h₁ <;> rename_i h₁ <;> apply h₁ x a <;> assumption
+
+end Cedar.Thm
