cedar-lean/Cedar/Thm/Validation/Typechecker/LitVar.lean
@@ -1,0 +1,73 @@
+/-
+ Copyright 2022-2023 Amazon.com, Inc. or its affiliates. All Rights Reserved.
+
+ Licensed under the Apache License, Version 2.0 (the "License");
+ you may not use this file except in compliance with the License.
+ You may obtain a copy of the License at
+
+      https://www.apache.org/licenses/LICENSE-2.0
+
+ Unless required by applicable law or agreed to in writing, software
+ distributed under the License is distributed on an "AS IS" BASIS,
+ WITHOUT WARRANTIES OR CONDITIONS OF ANY KIND, either express or implied.
+ See the License for the specific language governing permissions and
+ limitations under the License.
+-/
+
+import Cedar.Thm.Validation.Typechecker.Basic
+
+/-!
+This file proves that typechecking of `.lit` and `.var` expressions is sound.
+-/
+
+namespace Cedar.Thm
+
+open Cedar.Spec
+open Cedar.Validation
+
+theorem type_of_lit_is_sound {l : Prim} {c₁ c₂ : Capabilities} {env : Environment} {ty : CedarType} {request : Request} {entities : Entities}
+  (h₃ : typeOf (Expr.lit l) c₁ env = Except.ok (ty, c₂)) :
+  GuardedCapabilitiesInvariant (Expr.lit l) c₂ request entities ∧
+  ∃ v, EvaluatesTo (Expr.lit l) request entities v ∧ InstanceOfType v ty
+:= by
+  simp [EvaluatesTo, evaluate]
+  simp [typeOf, typeOfLit] at h₃
+  split at h₃ <;> simp [ok] at h₃
+  case h_5;
+  split at h₃ <;> try { simp [err] at h₃ }
+  simp at h₃
+  all_goals {
+    rcases h₃ with ⟨h₃, h₄⟩; rw [←h₃, ←h₄]; constructor
+    case left => exact empty_guarded_capabilities_invariant
+    case right => first |
+      exact true_is_instance_of_tt |
+      exact false_is_instance_of_ff |
+      apply InstanceOfType.instance_of_int |
+      apply InstanceOfType.instance_of_string |
+      apply InstanceOfType.instance_of_entity; simp [InstanceOfEntityType]
+  }
+
+theorem type_of_var_is_sound {var : Var} {c₁ c₂ : Capabilities} {env : Environment} {ty : CedarType} {request : Request} {entities : Entities}
+  (h₂ : RequestAndEntitiesMatchEnvironment env request entities)
+  (h₃ : typeOf (Expr.var var) c₁ env = Except.ok (ty, c₂)) :
+  GuardedCapabilitiesInvariant (Expr.var var) c₂ request entities ∧
+  ∃ v, EvaluatesTo (Expr.var var) request entities v ∧ InstanceOfType v ty
+:= by
+  simp [EvaluatesTo, evaluate]
+  simp [typeOf, typeOfVar] at h₃
+  rcases h₂ with ⟨h₂, _⟩
+  simp [InstanceOfRequestType] at h₂
+  split at h₃ <;> simp <;> simp [ok] at h₃ <;>
+  rcases h₃ with ⟨h₃, h₄⟩ <;> rw [←h₃, ←h₄] <;> constructor <;>
+  try { exact empty_guarded_capabilities_invariant }
+  case intro.h_1.intro.right =>
+    apply InstanceOfType.instance_of_entity; simp [h₂]
+  case intro.h_2.intro.right =>
+    apply InstanceOfType.instance_of_entity
+    simp [h₂, InstanceOfEntityType]
+  case intro.h_3.intro.right =>
+    apply InstanceOfType.instance_of_entity; simp [h₂]
+  case intro.h_4.intro.right =>
+    simp [h₂]
+
+end Cedar.Thm
