cedar-lean/Cedar/Thm/Validation/Typechecker/Or.lean
@@ -1,0 +1,172 @@
+/-
+ Copyright 2022-2023 Amazon.com, Inc. or its affiliates. All Rights Reserved.
+
+ Licensed under the Apache License, Version 2.0 (the "License");
+ you may not use this file except in compliance with the License.
+ You may obtain a copy of the License at
+
+      https://www.apache.org/licenses/LICENSE-2.0
+
+ Unless required by applicable law or agreed to in writing, software
+ distributed under the License is distributed on an "AS IS" BASIS,
+ WITHOUT WARRANTIES OR CONDITIONS OF ANY KIND, either express or implied.
+ See the License for the specific language governing permissions and
+ limitations under the License.
+-/
+
+import Cedar.Thm.Validation.Typechecker.Basic
+
+/-!
+This file proves that typechecking of `.or` expressions is sound.
+-/
+
+namespace Cedar.Thm
+
+open Cedar.Data
+open Cedar.Spec
+open Cedar.Validation
+
+theorem type_of_or_inversion {x₁ x₂ : Expr} {c c' : Capabilities} {env : Environment} {ty : CedarType}
+  (h₁ : typeOf (Expr.or x₁ x₂) c env = Except.ok (ty, c')) :
+  ∃ bty₁ c₁,
+    typeOf x₁ c env = .ok (.bool bty₁, c₁) ∧
+    if bty₁ = BoolType.tt
+    then ty = .bool BoolType.tt ∧ c' = ∅
+    else ∃ bty₂ c₂,
+      typeOf x₂ c env = .ok (.bool bty₂, c₂) ∧
+      if bty₁ = BoolType.ff
+      then ty = .bool bty₂ ∧ c' = c₂
+      else if bty₂ = BoolType.tt
+      then ty = .bool BoolType.tt ∧ c' = ∅
+      else if bty₂ = BoolType.ff
+      then ty = .bool BoolType.anyBool ∧ c' = c₁
+      else ty = .bool BoolType.anyBool ∧ c' = c₁ ∩ c₂
+:= by
+  simp [typeOf] at h₁
+  cases h₂ : typeOf x₁ c env <;> simp [h₂] at *
+  rename_i res₁
+  simp [typeOfOr] at h₁
+  split at h₁ <;> simp [ok, err] at h₁ <;>
+  rename_i hr₁ <;> simp at hr₁ <;>
+  rcases hr₁ with ⟨ht₁, hc₁⟩
+  case ok.h_1 c₁  =>
+    exists BoolType.tt, c₁
+    rcases h₁ with ⟨ht, hc⟩
+    simp [←ht₁, ←hc₁, hc, ←ht]
+  case ok.h_2 c₁ =>
+    cases h₃ : typeOf x₂ c env <;> simp [h₃] at *
+    rename_i res₂
+    split at h₁ <;> simp [ok, err] at h₁
+    rename_i bty₂ hr₂
+    rcases h₁ with ⟨ht, hc⟩ ; subst ht hc
+    exists BoolType.ff, c₁
+    simp [←ht₁, ←hc₁]
+    exists bty₂
+    simp [←hr₂]
+  case ok.h_3 bty₁ c₁ hneq₁ hneq₂ =>
+    cases bty₁ <;> simp at hneq₁ hneq₂
+    exists BoolType.anyBool, c₁
+    simp [←ht₁, ←hc₁]
+    cases h₃ : typeOf x₂ c env <;> simp [h₃] at *
+    rename_i res₂
+    split at h₁ <;> simp [ok, err] at h₁ <;>
+    rename_i hr₂ <;>
+    rcases h₁ with ⟨ht, hc⟩ <;> subst ht hc <;> simp
+    case h_1.intro =>
+      exists BoolType.tt, res₂.snd
+      simp [←hr₂]
+    case h_2.intro =>
+      exists BoolType.ff, res₂.snd
+      simp [←hr₂, ht₁, hc₁]
+    case h_3.intro bty₂ hneq₁ hneq₂ =>
+      exists bty₂, res₂.snd
+      simp [←hr₂, ←ht₁, ←hc₁]
+      cases bty₂ <;> simp at *
+
+theorem type_of_or_is_sound {x₁ x₂ : Expr} {c₁ c₂ : Capabilities} {env : Environment} {ty : CedarType} {request : Request} {entities : Entities}
+  (h₁ : CapabilitiesInvariant c₁ request entities)
+  (h₂ : RequestAndEntitiesMatchEnvironment env request entities)
+  (h₃ : typeOf (Expr.or x₁ x₂) c₁ env = Except.ok (ty, c₂))
+  (ih₁ : TypeOfIsSound x₁)
+  (ih₂ : TypeOfIsSound x₂) :
+  GuardedCapabilitiesInvariant (Expr.or x₁ x₂) c₂ request entities ∧
+  ∃ v, EvaluatesTo (Expr.or x₁ x₂) request entities v ∧ InstanceOfType v ty
+:= by
+  rcases (type_of_or_inversion h₃) with ⟨bty₁, rc₁, h₄, h₅⟩
+  specialize ih₁ h₁ h₂ h₄
+  rcases ih₁ with ⟨ih₁₁, v₁, ih₁₂, ih₁₃⟩
+  rcases (instance_of_bool_is_bool ih₁₃) with ⟨b₁, hb₁⟩ ; subst hb₁
+  split at h₅
+  case inl h₆ =>
+    subst h₆
+    rcases h₅ with ⟨hty, hc⟩ ; subst hty hc
+    apply And.intro
+    case left => exact empty_guarded_capabilities_invariant
+    case right =>
+      rcases (instance_of_tt_is_true ih₁₃) with h₇
+      simp at h₇ ; subst h₇
+      simp [EvaluatesTo] at ih₁₂
+      rcases ih₁₂ with ih₁₂ | ih₁₂ | ih₁₂ | ih₁₂ <;>
+      simp [EvaluatesTo, evaluate, Result.as, ih₁₂, Coe.coe, Value.asBool] <;>
+      try exact type_is_inhabited (CedarType.bool BoolType.tt)
+      exact true_is_instance_of_tt
+  case inr =>
+    rcases h₅ with ⟨bty₂, rc₂, h₅, h₇⟩
+    specialize ih₂ h₁ h₂ h₅
+    rcases ih₂ with ⟨ih₂₁, v₂, ih₂₂, ih₂₃⟩
+    rcases (instance_of_bool_is_bool ih₂₃) with ⟨b₂, hb₂⟩ ; subst hb₂
+    simp [EvaluatesTo]
+    cases b₁ <;>
+    rcases ih₁₂ with ih₁₂ | ih₁₂ | ih₁₂ | ih₁₂ <;>
+    rcases ih₂₂ with ih₂₂ | ih₂₂ | ih₂₂ | ih₂₂ <;>
+    simp [evaluate, Result.as, Coe.coe, Value.asBool, ih₁₂, ih₂₂, GuardedCapabilitiesInvariant] <;>
+    try exact type_is_inhabited ty
+    case false.inr.inr.inr.inr.inr.inr =>
+      cases b₂ <;> simp
+      case false h₆ =>
+        exists false ; simp only [true_and]
+        cases bty₁ <;> simp at h₆ h₇
+        case anyBool =>
+          cases bty₂ <;> simp at h₇ <;>
+          rcases h₇ with ⟨h₇, _⟩ <;> subst h₇ <;>
+          try exact bool_is_instance_of_anyBool false
+          exact ih₂₃
+        case ff => rcases h₇ with ⟨h₇, _⟩ ; subst h₇ ; exact ih₂₃
+      case true h₆ =>
+        cases bty₁ <;> cases bty₂ <;> simp at h₆ h₇ <;>
+        rcases h₇ with ⟨hty, hc⟩ <;> simp [hty, hc] at *
+        case ff.ff.intro => rcases ih₂₃ with ⟨_, _, ih₂₃⟩ ; simp [InstanceOfBoolType] at ih₂₃
+        case anyBool.ff.intro => rcases ih₂₃ with ⟨_, _, ih₂₃⟩ ; simp [InstanceOfBoolType] at ih₂₃
+        case anyBool.tt.intro =>
+          apply And.intro
+          case left => apply empty_capabilities_invariant
+          case right => exists true
+        case anyBool.anyBool.intro =>
+          apply And.intro
+          case left =>
+            simp [GuardedCapabilitiesInvariant, ih₂₂] at ih₂₁
+            apply capability_intersection_invariant
+            simp [ih₂₁]
+          case right => exists true
+        all_goals {
+          simp [GuardedCapabilitiesInvariant, ih₂₂] at ih₂₁
+          simp [ih₂₁]
+          exists true
+        }
+    all_goals {
+      simp [GuardedCapabilitiesInvariant] at ih₁₁ ih₂₁
+      simp [ih₁₂] at ih₁₁ ; simp [ih₂₂] at ih₂₁
+      rename_i h₆
+      rcases ih₁₃ with ⟨_, _, ih₁₃⟩ ; simp [InstanceOfBoolType] at ih₁₃
+      cases bty₁ <;> simp at h₆ ih₁₃ h₇
+      cases bty₂ <;> simp at h₇ <;>
+      rcases h₇ with ⟨ht, hc⟩ <;> simp [ht, hc] at * <;>
+      simp [true_is_instance_of_tt, bool_is_instance_of_anyBool] <;>
+      try { apply empty_capabilities_invariant } <;>
+      try { assumption }
+      apply capability_intersection_invariant
+      simp [ih₁₁, ih₂₁]
+    }
+
+
+end Cedar.Thm
