cedar-lean/Cedar/Thm/Validation/Typechecker/Set.lean
@@ -1,0 +1,290 @@
+/-
+ Copyright 2022-2023 Amazon.com, Inc. or its affiliates. All Rights Reserved.
+
+ Licensed under the Apache License, Version 2.0 (the "License");
+ you may not use this file except in compliance with the License.
+ You may obtain a copy of the License at
+
+      https://www.apache.org/licenses/LICENSE-2.0
+
+ Unless required by applicable law or agreed to in writing, software
+ distributed under the License is distributed on an "AS IS" BASIS,
+ WITHOUT WARRANTIES OR CONDITIONS OF ANY KIND, either express or implied.
+ See the License for the specific language governing permissions and
+ limitations under the License.
+-/
+
+import Cedar.Thm.Core.LT
+import Cedar.Thm.Validation.Typechecker.Basic
+
+/-!
+This file proves that typechecking of `.set` expressions is sound.
+-/
+
+namespace Cedar.Thm
+
+open Cedar.Data
+open Cedar.Spec
+open Cedar.Validation
+
+theorem lub_lub_fixed {ty₁ ty₂ ty₃ ty₄ : CedarType}
+  (h₁ : (ty₁ ⊔ ty₂) = some ty₃)
+  (h₂ : (ty₃ ⊔ ty₄) = some ty₄) :
+  (ty₁ ⊔ ty₄) = some ty₄
+:= by
+  rcases (lub_left_subty h₁) with h₃
+  rcases (lub_left_subty h₂) with h₄
+  rcases (subty_trans h₃ h₄) with h₅
+  simp [subty] at h₅
+  split at h₅ <;> simp at h₅ ; subst h₅
+  assumption
+
+theorem foldlM_of_lub_is_LUB {ty lubTy : CedarType } {tys : List CedarType}
+  (h₁ : List.foldlM lub? ty tys = some lubTy) :
+  (ty ⊔ lubTy) = some lubTy
+:= by
+  induction tys generalizing ty lubTy
+  case nil =>
+    simp [List.foldlM, pure] at h₁
+    subst h₁
+    exact lub_refl ty
+  case cons hd tl ih =>
+    simp [List.foldlM] at h₁
+    cases h₂ : ty ⊔ hd <;>
+    simp [h₂] at h₁
+    rename_i lubTy'
+    specialize ih h₁
+    apply lub_lub_fixed h₂ ih
+
+theorem foldlM_of_lub_assoc (ty₁ ty₂ : CedarType) (tys : List CedarType) :
+  List.foldlM lub? ty₁ (ty₂ :: tys) =
+  (do let ty₃ ← List.foldlM lub? ty₂ tys ; ty₁ ⊔ ty₃)
+:= by
+  apply List.foldlM_of_assoc
+  intro x₁ x₂ x₃
+  apply lub_assoc
+
+theorem type_of_set_tail
+  {x xhd : Expr } {xtl : List Expr} {c : Capabilities}
+  {env : Environment} {ty hd : CedarType } {tl : List CedarType}
+  (h₁ : (List.mapM₁ (xhd :: xtl) fun x => justType (typeOf x.val c env)) = Except.ok (hd :: tl))
+  (h₂ : List.foldlM lub? hd tl = some ty)
+  (h₃ : List.Mem x xtl) :
+  ∃ ty', typeOf (Expr.set xtl) c env = Except.ok (.set ty', []) ∧
+  (ty' ⊔ ty) = some ty
+:= by
+  cases xtl
+  case nil =>
+    rcases (List.not_mem_nil x) with _
+    contradiction
+  case cons xhd' xtl' =>
+    simp [typeOf]
+    cases tl
+    case nil =>
+      simp [List.mapM₁, List.attach] at h₁
+      simp [List.mapM_pmap_subtype (fun x => justType (typeOf x c env))] at h₁
+      cases h₄ : justType (typeOf xhd c env) <;> simp [h₄] at h₁
+      cases h₅ : justType (typeOf xhd' c env) <;> simp [h₅] at h₁
+      cases h₆ : List.mapM (fun x => justType (typeOf x c env)) xtl' <;> simp [h₆] at h₁
+      simp [pure, Except.pure] at h₁
+    case cons hd' tl' =>
+      simp [List.mapM₁] at h₁ ; unfold List.attach at h₁
+      rw [List.mapM_pmap_subtype (fun x => justType (typeOf x c env))] at h₁
+      rcases (List.mapM_head_tail h₁) with h₁
+      rw [←List.mapM₁_eq_mapM] at h₁
+      simp [h₁, typeOfSet]
+      cases h₄ : List.foldlM lub? hd' tl' <;>
+      simp [h₄, err, ok]
+      case none =>
+        rcases (foldlM_of_lub_assoc hd hd' tl') with h₅
+        rw [h₂, h₄] at h₅
+        simp at h₅
+      case some ty' =>
+        rcases (foldlM_of_lub_assoc hd hd' tl') with h₅
+        rw [h₂, h₄] at h₅
+        simp at h₅ ; rw [eq_comm, lub_comm] at h₅
+        rcases (lub_left_subty h₅) with h₆
+        simp [subty] at h₆
+        split at h₆ <;> simp at h₆
+        subst h₆
+        assumption
+
+theorem type_of_set_inversion {xs : List Expr} {c c' : Capabilities} {env : Environment} {sty : CedarType}
+  (h₁ : typeOf (Expr.set xs) c env = Except.ok (sty, c')) :
+  c' = ∅ ∧
+  ∃ ty,
+    sty = .set ty ∧
+    ∀ xᵢ, xᵢ ∈ xs →
+      ∃ tyᵢ cᵢ,
+        typeOf xᵢ c env = Except.ok (tyᵢ, cᵢ) ∧
+        (tyᵢ ⊔ ty) = .some ty
+:= by
+  simp [typeOf] at h₁
+  cases h₂ : List.mapM₁ xs fun x => justType (typeOf x.val c env) <;>
+  simp [h₂] at h₁
+  simp [typeOfSet] at h₁
+  split at h₁ <;> simp [ok, err] at h₁
+  rename_i hd tl
+  split at h₁ <;> simp at h₁
+  rename_i ty h₃
+  rcases h₁ with ⟨hl₁, hr₁⟩
+  subst hl₁ hr₁ ; simp only [true_and]
+  exists ty ; simp only [exists_and_right, true_and]
+  intro x h₄
+  cases h₄
+  case head xtl =>
+    simp [List.mapM₁, List.attach] at h₂
+    rcases h₅ : justType (typeOf x c env) <;>
+    simp [h₅] at h₂
+    simp [List.mapM_pmap_subtype (fun x => justType (typeOf x c env))] at h₂
+    rcases h₆ : List.mapM (fun x => justType (typeOf x c env)) xtl <;>
+    simp [h₆, pure, Except.pure] at h₂
+    rcases h₂ with ⟨hl₂, hr₂⟩ ; subst hl₂ hr₂
+    rename_i hdty tlty
+    simp [justType, Except.map] at h₅
+    split at h₅ <;> simp at h₅
+    rename_i res h₇
+    exists hdty
+    apply And.intro
+    case left =>
+      exists res.snd
+      simp [←h₅, h₇]
+    case right =>
+      exact foldlM_of_lub_is_LUB h₃
+  case tail xhd xtl h₄ =>
+    rcases (type_of_set_tail h₂ h₃ h₄) with ⟨ty', h₅, h₆⟩
+    rcases (@type_of_set_inversion xtl c ∅ env (.set ty')) with h₇
+    simp [h₅] at h₇
+    specialize h₇ x h₄
+    rcases h₇ with ⟨tyᵢ, h₇, h₈⟩
+    exists tyᵢ
+    rcases h₇ with ⟨cᵢ, h₇⟩
+    apply And.intro
+    case left  => exists cᵢ
+    case right => apply lub_lub_fixed h₈ h₆
+
+theorem list_is_sound_implies_tail_is_sound {hd : Expr} {tl : List Expr}
+  (h₁ : ∀ (xᵢ : Expr), xᵢ ∈ hd :: tl → TypeOfIsSound xᵢ) :
+  ∀ (xᵢ : Expr), xᵢ ∈ tl → TypeOfIsSound xᵢ
+:= by
+  intro xᵢ h₂
+  apply h₁
+  simp [h₂]
+
+theorem list_is_typed_implies_tail_is_typed {hd : Expr} {tl : List Expr} {c₁ : Capabilities} {env : Environment} {ty : CedarType}
+  (h₁ : ∀ (xᵢ : Expr), xᵢ ∈ hd :: tl → ∃ tyᵢ cᵢ, typeOf xᵢ c₁ env = Except.ok (tyᵢ, cᵢ) ∧ (tyᵢ ⊔ ty) = some ty) :
+  ∀ (xᵢ : Expr), xᵢ ∈ tl → ∃ tyᵢ cᵢ, typeOf xᵢ c₁ env = Except.ok (tyᵢ, cᵢ) ∧ (tyᵢ ⊔ ty) = some ty
+:= by
+  intro xᵢ h₂
+  apply h₁
+  simp [h₂]
+
+theorem type_of_set_is_sound_err {xs : List Expr} {c₁ : Capabilities} {env : Environment} {ty : CedarType} {request : Request} {entities : Entities} {err : Error}
+  (ih : ∀ (xᵢ : Expr), xᵢ ∈ xs → TypeOfIsSound xᵢ)
+  (h₁ : CapabilitiesInvariant c₁ request entities)
+  (h₂ : RequestAndEntitiesMatchEnvironment env request entities)
+  (h₄ : ∀ (xᵢ : Expr), xᵢ ∈ xs → ∃ tyᵢ cᵢ, typeOf xᵢ c₁ env = Except.ok (tyᵢ, cᵢ) ∧ (tyᵢ ⊔ ty) = some ty)
+  (h₅ : (xs.mapM fun x => evaluate x request entities) = Except.error err) :
+  err = Error.entityDoesNotExist ∨
+  err = Error.extensionError ∨
+  err = Error.arithBoundsError
+:= by
+  cases h₆ : xs
+  case nil =>
+    subst h₆
+    simp [List.mapM₁, List.attach, pure, Except.pure] at h₅
+  case cons hd tl =>
+    simp [List.mapM₁, List.attach, h₆] at h₅
+    rcases (h₄ hd) with h₄
+    simp only [h₆, List.mem_cons, true_or, forall_const] at h₄
+    rcases h₄ with ⟨tyᵢ, cᵢ, h₇, _⟩
+    rcases (ih hd) with h₉ ; simp [h₆, TypeOfIsSound] at h₉
+    specialize (h₉ h₁ h₂ h₇) ; rcases h₉ with ⟨_, v, h₉⟩
+    simp [EvaluatesTo] at h₉
+    rcases h₉ with ⟨h₉, _⟩
+    rcases h₉ with h₉ | h₉ | h₉ | h₉ <;>
+    simp [h₉] at h₅ <;>
+    try { simp [h₅] }
+    subst h₆
+    cases h₁₀ : List.mapM (fun x => evaluate x request entities) tl <;>
+    simp [h₁₀, pure, Except.pure] at h₅ ; rw [eq_comm] at h₅
+    subst h₅
+    apply @type_of_set_is_sound_err
+      tl c₁ env ty request entities err
+      (list_is_sound_implies_tail_is_sound ih)
+      h₁ h₂
+      (list_is_typed_implies_tail_is_typed h₄)
+    exact h₁₀
+
+theorem type_of_set_is_sound_ok { xs : List Expr } { c₁ : Capabilities } { env : Environment } { request : Request } { entities : Entities } { ty : CedarType } { v : Value } { vs : List Value }
+  (ih : ∀ (xᵢ : Expr), xᵢ ∈ xs → TypeOfIsSound xᵢ)
+  (h₁ : CapabilitiesInvariant c₁ request entities)
+  (h₂ : RequestAndEntitiesMatchEnvironment env request entities)
+  (h₃ : ∀ (xᵢ : Expr), xᵢ ∈ xs → ∃ tyᵢ cᵢ, typeOf xᵢ c₁ env = Except.ok (tyᵢ, cᵢ) ∧ (tyᵢ ⊔ ty) = some ty)
+  (h₄ : (xs.mapM fun x => evaluate x request entities) = Except.ok vs)
+  (h₅ : v ∈ vs):
+  InstanceOfType v ty
+:= by
+  cases xs
+  case nil =>
+    simp [List.mapM₁, List.attach, pure, Except.pure] at h₄
+    subst h₄
+    simp only [List.find?_nil, List.not_mem_nil] at h₅
+  case cons hd tl =>
+    simp [List.mapM₁, List.attach] at h₄
+    cases h₇ : evaluate hd request entities <;>
+    simp [h₇] at h₄
+    rename_i vhd
+    cases h₈ : List.mapM (fun x => evaluate x request entities) tl <;>
+    simp [h₈, pure, Except.pure] at h₄
+    rename_i vtl
+    subst h₄
+    cases h₅
+    case head =>
+      specialize h₃ hd
+      simp only [List.mem_cons, true_or, forall_const] at h₃
+      rcases h₃ with ⟨tyᵢ, cᵢ, h₃, h₆⟩
+      specialize ih hd
+      simp [TypeOfIsSound] at ih
+      specialize ih h₁ h₂ h₃
+      rcases ih with ⟨_, v', ihl, ihr⟩
+      simp [EvaluatesTo] at ihl
+      rcases ihl with ihl | ihl | ihl | ihl <;>
+      simp [ihl] at h₇
+      subst h₇
+      exact instance_of_lub_left h₆ ihr
+    case tail h₉ =>
+      apply @type_of_set_is_sound_ok
+        tl c₁ env request entities ty v vtl
+        (list_is_sound_implies_tail_is_sound ih)
+        h₁ h₂
+        (list_is_typed_implies_tail_is_typed h₃)
+        _ h₉
+      simp [List.mapM₁, List.attach, List.mapM_pmap_subtype (evaluate · request entities), h₈]
+
+theorem type_of_set_is_sound {xs : List Expr} {c₁ c₂ : Capabilities} {env : Environment} {sty : CedarType} {request : Request} {entities : Entities}
+  (h₁ : CapabilitiesInvariant c₁ request entities)
+  (h₂ : RequestAndEntitiesMatchEnvironment env request entities)
+  (h₃ : typeOf (Expr.set xs) c₁ env = Except.ok (sty, c₂))
+  (ih : ∀ (xᵢ : Expr), xᵢ ∈ xs → TypeOfIsSound xᵢ) :
+  GuardedCapabilitiesInvariant (Expr.set xs) c₂ request entities ∧
+  ∃ v, EvaluatesTo (Expr.set xs) request entities v ∧ InstanceOfType v sty
+:= by
+  rcases (type_of_set_inversion h₃) with ⟨h₆, ty, h₄, h₅⟩
+  subst h₆ h₄
+  apply And.intro
+  case left => exact empty_guarded_capabilities_invariant
+  case right =>
+    simp [EvaluatesTo, evaluate, List.mapM₁, List.attach, List.mapM_pmap_subtype (evaluate · request entities)]
+    cases h₆ : xs.mapM fun x => evaluate x request entities <;>
+    simp [h₆]
+    case error err =>
+      simp [type_is_inhabited]
+      exact type_of_set_is_sound_err ih h₁ h₂ h₅ h₆
+    case ok vs =>
+      apply InstanceOfType.instance_of_set
+      intro v h₇
+      rw [←Set.make_mem] at h₇
+      exact type_of_set_is_sound_ok ih h₁ h₂ h₅ h₆ h₇
+
+end Cedar.Thm
